@prefix dct: <http://purl.org/dc/terms/> .
@prefix pav: <http://purl.org/pav/> .
@prefix rdf: <http://www.w3.org/1999/02/22-rdf-syntax-ns#> .
@prefix skos: <http://www.w3.org/2004/02/skos/core#> .
@prefix temp-vocab: <http://www.fairdatacollective.com/template-vocabulary/> .

<http://www.fairdatacollective.com/template-vocabulary/> a skos:ConceptScheme;
  dct:contributor <https://orcid.org/0000-0001-6875-5360>;
  dct:creator <https://orcid.org/0000-0002-9381-9694>;
  dct:description "This is a template for building SKOS based controlled vocabulary which is used as base of the worflow describe in excel2rdf.readthedocs.io/"@en;
  dct:title "Template for building SKOS based controlled vocabulary"@en;
  pav:createdOn "2020-10-22T22:00:00+01:00"@en;
  pav:lastUpdatedOn "2020-10-23T08:00:00+01:00"@en;
  pav:version "0.1"@en;
  skos:hasTopConcept temp-vocab:TopConceptTwo, temp-vocab:TopConcetOne;
  skos:prefLabel "Template for building SKOS based controlled vocabulary"@en .

temp-vocab:TopConcetOne a skos:Concept;
  dct:contributor <https://orcid.org/0000-0001-6875-5360>;
  dct:creator <https://orcid.org/0000-0002-9381-9693>;
  skos:definition "This is a top concept which is used to collect a number of narrower concepts."@en;
  skos:inScheme <http://www.fairdatacollective.com/template-vocabulary/>;
  skos:narrower temp-vocab:NarrowConceptOne;
  skos:prefLabel "TopConcetOne"@en;
  skos:topConceptOf <http://www.fairdatacollective.com/template-vocabulary/> .

temp-vocab:TopConceptTwo a skos:Concept;
  dct:contributor <https://orcid.org/0000-0001-6875-5360>;
  dct:creator <https://orcid.org/0000-0002-9381-9693>;
  skos:definition "This is yet another top concept which is used to collect a number of narrower concepts."@en;
  skos:inScheme <http://www.fairdatacollective.com/template-vocabulary/>;
  skos:narrower temp-vocab:NarrowConceptTwo;
  skos:prefLabel "TopConceptTwo"@en;
  skos:topConceptOf <http://www.fairdatacollective.com/template-vocabulary/> .

temp-vocab:NarrowConceptOne a skos:Concept;
  dct:contributor <https://orcid.org/0000-0001-6875-5360>;
  dct:creator <https://orcid.org/0000-0002-9381-9693>;
  skos:broader temp-vocab:TopConcetOne;
  skos:definition "A definition of NarrowConceptOne, which has a broader concept TopConceptOne."@en;
  skos:inScheme <http://www.fairdatacollective.com/template-vocabulary/>;
  skos:prefLabel "NarrowConceptOne"@en .

temp-vocab:NarrowConceptTwo a skos:Concept;
  dct:contributor <https://orcid.org/0000-0001-6875-5360>;
  dct:creator <https://orcid.org/0000-0002-9381-9693>;
  skos:broader temp-vocab:TopConceptTwo;
  skos:definition "A definition of NarrowConceptTwo, which has a broader concept TopConceptTwo."@en;
  skos:inScheme <http://www.fairdatacollective.com/template-vocabulary/>;
  skos:prefLabel "NarrowConceptTwo"@en .
